Execution_resources/lemmas.v
@@ -1,90 +1,8 @@
 
 From Views Require Import utils.
 From Views.Execution_resources Require Import Execution_resources.
+From Views.Execution_resources Require Import sets_of_threads.
 Require Import PeanoNat.
-
-
-Fixpoint thread_set_1z {T : Type} (x y z : nat) (f : T -> List ThreadId_t) : Tensor T (x,y,z) -> List ThreadId_t :=
-  match (x,y,z) with
-  | (S x, S y, S z) =>
-      fun m => f (m x y z) ++ (thread_set_1z (S x) (S y) z f m)
-  | _ => fun _ => []
-end.
-
-
-Fixpoint thread_set_1y {T : Type} (x y z : nat) (f : T -> List ThreadId_t) : Tensor T (x,y,z) -> List ThreadId_t :=
-  match (x,y,z) with
-  | (S x, S y, S z) =>
-      fun m => f (m x y z) ++ (thread_set_1y (S x) y (S z) f m)
-  | _ => fun _ => []
-end.
-
-Fixpoint thread_set_2yz {T : Type} (x y z : nat) (f : T -> List ThreadId_t) : Tensor T (x,y,z) -> List ThreadId_t :=
-  match (x,y,z) with
-  | (S x, S y, S z) =>
-      fun m => thread_set_1z (S x) (S y) (S z) f m  ++ (thread_set_2yz (S x) y (S z) f m) 
-  | _ => fun _ => []
-end.
-
-Fixpoint thread_set_2xz {T : Type} (x y z : nat) (f : T -> List ThreadId_t) : Tensor T (x,y,z) -> List ThreadId_t :=
-  match (x,y,z) with
-  | (S x, S y, S z) =>
-      fun m => thread_set_1z (S x) (S y) (S z) f m  ++ (thread_set_2xz x (S y) (S z) f m) 
-  | _ => fun _ => []
-end.
-
-Fixpoint thread_set_2xy {T : Type} (x y z : nat) (f : T -> List ThreadId_t) : Tensor T (x,y,z) -> List ThreadId_t :=
-  match (x,y,z) with
-  | (S x, S y, S z) =>
-      fun m => thread_set_1y (S x) (S y) (S z) f m  ++ (thread_set_2xy x (S y) (S z) f m) 
-  | _ => fun _ => []
-end.
-
-Fixpoint thread_set_3xyz {T : Type} (x y z : nat) (f : T -> List ThreadId_t) : Tensor T (x,y,z) -> List ThreadId_t :=
-  match (x,y,z) with
-  | (S x, S y, S z) =>
-         fun m => thread_set_2yz (S x) (S y) (S z) f m ++ (thread_set_3xyz x (S y) (S z) f m) 
-  | _ => fun _ => []
-end.
-
-Fixpoint thread_set_3yxz {T : Type} (x y z : nat) (f : T -> List ThreadId_t) : Tensor T (x,y,z) -> List ThreadId_t :=
-  match (x,y,z) with
-  | (S x, S y, S z) =>
-         fun m => thread_set_2xz (S x) (S y) (S z) f m ++ (thread_set_3yxz (S x) y (S z) f m) 
-  | _ => fun _ => []
-end.
-
-Fixpoint thread_set_3zxy {T : Type} (x y z : nat) (f : T -> List ThreadId_t) : Tensor T (x,y,z) -> List ThreadId_t :=
-  match (x,y,z) with
-  | (S x, S y, S z) =>
-         fun m => thread_set_2xy (S x) (S y) (S z) f m ++ (thread_set_3zxy (S x) (S y) z f m) 
-  | _ => fun _ => []
-end.
-
-Fixpoint thread_set' (e : execution_resource) : List ThreadId_t :=
-  match e with
-  | Collection n v => zip (buildList n (fun i => thread_set' (v i)))
-  | grid (x,y,z) (x',y',z') g => thread_set_3xyz x y z (fun b => thread_set_3xyz x' y' z' (fun x => x :: []) b) g
-  | block (x,y,z) _ b => thread_set_3xyz x y z (fun x => x :: []) b
-  | lthread i => i::[]
-  | _ => []
-end.
-
-(** TODO : add physical address translation of blocks, grids and lthreads *)
-Fixpoint physical_thread_set (e : execution_resource) (f : ThreadId_t -> PhysicalId_t) : List PhysicalId_t :=
-  match e with
-  | Collection n v => zip (buildList n (fun i => physical_thread_set (v i) f))
-  | thread i => i::[]
-  | warp w => buildList Warp_size (fun i => w i)
-  | _ => []
-end.
-
-
-Inductive count {T : Type} : T -> List T -> nat -> Prop :=
-  | empty (x : T) : count x [] 0
-  | cons_eq (x : T) (tl : List T) {n : nat} (H : count x tl n) : count x (x::tl) (S n)
-  | cons_neq (x : T) (y : T) (tl : List T) {n : nat} (H : count x tl n) (Hneq : x <> y) : count x (y::tl) n
-.
 
 Lemma cat_count :
   forall T l1 l2 (x : T) m n,
@@ -305,4 +223,57 @@ Proof.
   intros. induction n.
   - reflexivity.
   - simpl. rewrite map_cat. rewrite IHn. reflexivity.
+Qed.
+
+Fixpoint eqb (m n : nat) :=
+  match m,n with
+  | 0,0 => true
+  | S m, S n => eqb m n
+  | _,_ => false
+end.
+
+Fixpoint sum {n : nat} (v : Vector nat n) :=
+  match n with
+  | 0 => 0
+  | S n => v n + sum v (n := n)
+end.
+
+Proposition eqb_correct :
+  forall m n, eqb m n = true -> m = n
+.
+Proof.
+  induction m.
+  - destruct n. reflexivity. intro. inversion H.
+  - destruct n. intro. inversion H. intro. apply IHm in H. subst; reflexivity.
+Qed.
+
+Proposition eqb_correct_2 :
+  forall m n, m <> n -> eqb m n = false
+.
+Proof.
+  induction m.
+  - destruct n. intro. exfalso. apply H. reflexivity. reflexivity.
+  - destruct n. reflexivity. intro. apply IHm. intro. rewrite H0 in H. apply H. reflexivity.
+Qed.
+
+Proposition eqb_refl :
+  forall n, eqb n n = true
+.
+Proof.
+  induction n.
+  - reflexivity.
+  - apply IHn.
+Qed.
+
+Proposition vector_sum_eq :
+  forall n (v1 v2 : Vector nat n),
+  (forall i, i < n -> v1 i = v2 i) -> sum v1 = sum v2.
+Proof.
+  induction n.
+  - reflexivity.
+  - intros. simpl. assert (forall i : nat, i < n -> v1 i = v2 i).
+    intros. apply le_S in H0. apply H in H0. apply H0.
+    apply IHn in H0. rewrite H0.
+    assert (v1 n = v2 n). apply H. apply le_n. rewrite H1.
+    reflexivity.
 Qed.
