Execution_resources/blocks.v
@@ -2,6 +2,7 @@
 From Views Require Import utils.
 From Views.Execution_resources Require Import Execution_resources.
 From Views.Execution_resources Require Import lemmas.
+From Views.Execution_resources Require Import sets_of_threads.
 Require Import PeanoNat.
 
 Proposition block_not_contain_larger_on_z :
