Execution_resources/collections.v
@@ -1,0 +1,36 @@
+
+From Views Require Import utils.
+From Views.Execution_resources Require Import Execution_resources.
+From Views.Execution_resources Require Import lemmas.
+From Views.Execution_resources Require Import correctness_lemmas.
+From Views.Execution_resources Require Import sets_of_threads.
+Require Import PeanoNat.
+
+Proposition collection_correct :
+  forall a n (v : Vector execution_resource n),
+      exists (m : Vector nat n), (forall i, i < n -> count a (thread_set' (v i)) (m i)) ->
+      count a (thread_set' (Collection n v)) (sum m)
+.
+Proof.
+  induction n.
+    - exists (fun i => i). intros. apply empty.
+    - intros. assert (exists m : Vector nat n,
+        (forall i : nat, i < n -> count a (thread_set' (v i)) (m i)) ->
+        count a (thread_set' (Collection n v)) (sum m)). apply IHn.
+      destruct H.
+      assert (exists m, count a (thread_set' (v n)) m). apply count_exists.
+      destruct H0.
+      exists (fun i => if (eqb i n) then x0 else x i).
+      intros.
+      simpl. apply cat_count.
+      * rewrite eqb_refl. apply H0.
+      * assert (sum (n := n) (fun i : nat => if eqb i n then x0 else x i) = sum x).
+        apply vector_sum_eq.
+        intros. assert (eqb i n = false). apply eqb_correct_2.
+        intro. subst. apply Nat.lt_irrefl in H2. apply H2. rewrite H3. reflexivity.
+        rewrite H2. apply H.
+        intros. assert (i < (S n)). apply le_S in H3. apply H3.
+        apply H1 in H4. assert (eqb i n = false). apply eqb_correct_2.
+        intro. subst. apply Nat.lt_irrefl in H3. apply H3. rewrite H5 in H4.
+        apply H4.
+Qed.
